theories/RocqsheetCofix.v
@@ -155,6 +155,11 @@ Definition trans (st : State) : State + option Z :=
   | PCEval _ (ESumIf _ _ _ _ _) => inr None
   | PCEval _ (ECountIf _ _ _ _) => inr None
   | PCEval _ (EAvgIf _ _ _ _ _) => inr None
+  (* Item 27: statistics bail out the same way. *)
+  | PCEval _ (EVarSamp _ _) => inr None
+  | PCEval _ (EVarPop _ _) => inr None
+  | PCEval _ (EStdevSamp _ _) => inr None
+  | PCEval _ (EStdevPop _ _) => inr None
   | PCSumStep visited lc hc col row hr acc =>
       if PrimInt63.ltb hr row then
         inl (mkSt (st_sheet st) (PCApply (Some acc)) (st_stack st))
